experiments with functors

theories/Cleanup.v
@@ -1,24 +1,23 @@
-From Prototype Require Import Prelude Sig LevelTwo.
-From Prototype Require LevelOne.
-Module O := LevelOne.
+From Prototype Require Import Prelude Sig ExplicitSyntax.
 
-(** The output of simplification (LevelTwoSimp.v) is good for comparing
-    terms/equations for equality, but not very nice to work with. 
+(** The output of simplification (Simplification.v) is good for comparing
+    terms/substitutions for equality, but not very nice to work with for the user. 
     This file implements cleanup functions which do trivial transformations 
     such as turning [Q_rapply R_shift i] into [Q_succ i], and are 
-    typically applied after simplification. Cleanup functions can be applied to all terms (not only the output 
-    of [LevelTwoSimp.v].
+    typically applied after simplification. 
+    Cleanup functions can be applied to all terms (not only the output 
+    of [Simplification.v].
     
     We formulate the correctness of cleanup as a rewriting system 
     ([qred], [rred], [ered], [sred]), which is proved correct with 
     respect to evaluation (lemmas [ered_sound], [sred_sound], etc).
     Contrary to simplification, we don't prove that we obtain
-    irreducible forms (for the cleanup rewriting system), although
-    we conjecture that it is true.  *)
+    irreducible forms (for the cleanup rewriting system) because it is
+    too much effort, although we might do the proofs in the future.
+*)
 
 Section WithSignature.
 Context {sig : signature}.
-#[local] Existing Instance sig.
 
 (*********************************************************************************)
 (** *** [mk_qsucc] *)
@@ -33,7 +32,7 @@ mk_qsucc (S n) i := Q_succ (mk_qsucc n i).
 Lemma eval_mk_qsucc e n i :
   qeval e (mk_qsucc n i) = S n + qeval e i.
 Proof.
-funelim (mk_qsucc n i) ; simp mk_qsucc qeval ; triv.
+funelim (mk_qsucc n i) ; simp mk_qsucc qeval ; auto.
 rewrite H. lia. 
 Qed.
 #[local] Hint Rewrite eval_mk_qsucc : qeval.
@@ -57,10 +56,10 @@ dest_rshift _ := None.
 Lemma dest_rshift_sound e r n : 
   dest_rshift r = Some n -> reval e r =₁ add (S n).
 Proof.
-funelim (dest_rshift r) ; simp dest_rshift in * ; triv.
+funelim (dest_rshift r) ; simp dest_rshift in * ; try easy.
 - intros H. depelim H. reflexivity.
 - intros H. depelim H. simp qeval. apply (Hind e n2) in Heq. rewrite Heq. 
-  apply (Hind0 e n1) in Heq0. rewrite Heq0. cbv [P.rcomp]. intros i. lia.
+  apply (Hind0 e n1) in Heq0. rewrite Heq0. cbv [Prelude.rcomp]. intros i. lia.
 Qed.
 
 (*********************************************************************************)
@@ -70,7 +69,7 @@ Qed.
 Equations dest_ren (s : subst) : option ren :=
 dest_ren S_id := Some R_id ;
 dest_ren S_shift := Some R_shift ;
-dest_ren (S_cons (E_tvar i) s) with dest_ren s := {
+dest_ren (S_cons (E_var i) s) with dest_ren s := {
   | Some r => Some (R_cons i r) 
   | _ => None 
   } ;
@@ -84,36 +83,14 @@ dest_ren _ := None.
 Lemma dest_ren_sound e s r : 
   dest_ren s = Some r -> seval e s =₁ seval e (S_ren r).
 Proof.
-funelim (dest_ren s) ; triv.
+funelim (dest_ren s).
 all: intros H ; depelim H ; simp eeval qeval in * ; try reflexivity.
 - rewrite (Hind e r Heq). simp eeval. intros [|] ; reflexivity.
 - rewrite (Hind e r2 Heq), (Hind0 e r1 Heq0). reflexivity.
 Qed.
 
 (*********************************************************************************)
-(** *** Core rewriting system. *)
-(*********************************************************************************)
-
-#[local] Reserved Notation "i '=q=>₁' i'" (at level 70, no associativity). 
-#[local] Reserved Notation "e '=e=>₁' e'" (at level 70, no associativity). 
-
-Inductive qred1 : qnat -> qnat -> Prop :=
-| qred1_rapply_shift r i n : dest_rshift r = Some n -> Q_rapply r i =q=>₁ mk_qsucc n i
-where "i '=q=>₁' i'" := (qred1 i i').
-
-Inductive ered1 : forall {k}, expr k -> expr k -> Prop :=
-| ered1_ren_var r i : E_ren r (E_tvar i) =e=>₁ E_tvar (Q_rapply r i)
-| ered1_subst_ren {k} s r (t : expr k) : dest_ren s = Some r -> E_subst s t =e=>₁ E_ren r t
-| ered1_subst_var s i : E_subst s (E_tvar i) =e=>₁ E_sapply s i
-| ered1_sapply_ren s r i : dest_ren s = Some r -> E_sapply s i =e=>₁ E_ren r (E_tvar i)
-where "t =e=>₁ t'" := (ered1 t t').
-
-#[local] Hint Constructors qred1 ered1 : core.
-
-Derive Signature for qred1 ered1.
-
-(*********************************************************************************)
-(** *** Full rewriting system. *)
+(** *** Rewriting system. *)
 (*********************************************************************************)
 
 #[local] Reserved Notation "i =q=> i'" (at level 70, no associativity). 
@@ -130,8 +107,8 @@ Inductive qred : qnat -> qnat -> Prop :=
 (* Congruence. *)
 | qred_congr_succ : Proper (qred ==> qred) Q_succ
 | qred_congr_rapply : Proper (rred ==> qred ==> qred) Q_rapply 
-(* Core rules. *)
-| qred_core i i' : i =q=>₁ i' -> i =q=> i'
+(* Cleanup rules. *)
+| qred_rapply_shift r i n : dest_rshift r = Some n -> Q_rapply r i =q=> mk_qsucc n i
 
 with rred : ren -> ren -> Prop :=
 (* Preorder. *)
@@ -149,16 +126,20 @@ Inductive ered : forall {k}, expr k -> expr k -> Prop :=
 | ered_refl {k} : reflexive (expr k) ered
 | ered_trans {k} : transitive (expr k) ered
 (* Congruence. *)
-| ered_congr_tvar : Proper (qred ==> ered) E_tvar
-| ered_congr_tctor c : Proper (ered ==> ered) (E_tctor c)
+| ered_congr_tvar : Proper (qred ==> ered) E_var
+| ered_congr_tctor c : Proper (ered ==> ered) (E_ctor c)
 | ered_congr_al_cons {ty tys} : Proper (ered ==> ered ==> ered) (@E_al_cons _ ty tys)
 | ered_congr_aterm : Proper (ered ==> ered) E_aterm
 | ered_congr_abind {ty} : Proper (ered ==> ered) (@E_abind _ ty)
+| ered_congr_afunctor {ty} f sh : Proper (vec_eq ered ==> ered) (@E_afunctor _ ty f sh)
 | ered_congr_sapply : Proper (sred ==> qred ==> ered) E_sapply
 | ered_congr_ren {k} : Proper (rred ==> ered ==> ered) (@E_ren _ k)
 | ered_congr_subst {k} : Proper (sred ==> ered ==> ered) (@E_subst _ k)
-(* Core rules. *)
-| ered_core {k} (t t' : expr k) : t =e=>₁ t' -> t =e=> t'
+(* Cleanup rules. *)
+| ered_ren_var r i : E_ren r (E_var i) =e=> E_var (Q_rapply r i)
+| ered_subst_ren {k} s r (t : expr k) : dest_ren s = Some r -> E_subst s t =e=> E_ren r t
+| ered_subst_var s i : E_subst s (E_var i) =e=> E_sapply s i
+| ered_sapply_ren s r i : dest_ren s = Some r -> E_sapply s i =e=> E_ren r (E_var i)
 
 with sred : subst -> subst -> Prop :=
 (* Preorder. *)
@@ -191,13 +172,13 @@ Combined Scheme ered_sred_ind from ered_ind, sred_ind.
 (*********************************************************************************)
 
 #[export] Instance qred_preorder : PreOrder qred.
-Proof. constructor ; triv. Qed.
+Proof. constructor ; eauto. Qed.
 #[export] Instance rred_preorder : PreOrder rred.
-Proof. constructor ; triv. Qed.
+Proof. constructor ; eauto. Qed.
 #[export] Instance ered_preorder k : PreOrder (@ered k).
 Proof. constructor ; [apply ered_refl | apply ered_trans]. Qed.
 #[export] Instance sred_preorder : PreOrder sred.
-Proof. constructor ; triv. Qed.
+Proof. constructor ; eauto. Qed.
 
 #[export] Existing Instance qred_congr_succ.
 #[export] Existing Instance qred_congr_rapply.
@@ -208,6 +189,7 @@ Proof. constructor ; triv. Qed.
 #[export] Existing Instance ered_congr_al_cons.
 #[export] Existing Instance ered_congr_aterm.
 #[export] Existing Instance ered_congr_abind.
+#[export] Existing Instance ered_congr_afunctor.
 #[export] Existing Instance ered_congr_sapply.
 #[export] Existing Instance ered_congr_ren.
 #[export] Existing Instance ered_congr_subst.
@@ -223,10 +205,11 @@ Lemma qred_rred_sound e :
   (forall i i', i =q=> i' -> qeval e i = qeval e i') /\
   (forall r r', r =r=> r' -> reval e r =₁ reval e r').
 Proof.
-apply qred_rred_ind ; intros ; simp qeval ; triv.
+apply qred_rred_ind ; intros ; simp qeval ; auto.
 - now rewrite H0, H2.
 - now rewrite H0, H2.
-- depelim H. simp qeval. now rewrite (dest_rshift_sound _ _ _ H).
+- now rewrite (dest_rshift_sound _ _ _ H).
+- reflexivity.
 - now rewrite H0.
 - now rewrite H0, H2.
 - now rewrite H0, H2.
@@ -242,15 +225,16 @@ Lemma ered_sred_sound e :
   (forall {k} (t t' : expr k), t =e=> t' -> eeval e t = eeval e t') /\
   (forall s s', s =s=> s' -> seval e s =₁ seval e s').
 Proof.
-apply ered_sred_ind ; intros ; simp eeval ; triv.
-all: try solve [ now rewrite H0, H2 ].
+apply ered_sred_ind ; intros ; simp eeval ; auto.
+all: try solve [ now rewrite H0 | now rewrite H0, H2 ].
 - eapply qred_sound in H. now rewrite H.
+- f_equal. apply vec_ext. intros i. simp vec_nth.
 - eapply qred_sound in H1. now rewrite H0, H1.
 - eapply rred_sound in H. now rewrite H1, H.
-- depelim H ; simp eeval ; triv.
-  + eapply dest_ren_sound in H. rewrite H. simp eeval.
-    now rewrite O.ren_is_subst.
-  + eapply dest_ren_sound in H. rewrite H. simp eeval. simp rename. reflexivity.
+- eapply dest_ren_sound in H. rewrite H. simp eeval.
+  now rewrite P.ren_is_subst.
+- eapply dest_ren_sound in H. rewrite H. simp eeval. simp rename. reflexivity.
+- reflexivity.
 - eapply rred_sound in H. now rewrite H.
 Qed.
 
@@ -259,7 +243,7 @@ Proof. now apply ered_sred_sound. Qed.
 
 Lemma sred_sound e s s' : s =s=> s' -> seval e s =₁ seval e s'.
 Proof. now apply ered_sred_sound. Qed.
- 
+
 (*********************************************************************************)
 (** *** [rapply]. *)
 (*********************************************************************************)
@@ -272,7 +256,7 @@ rapply r i with dest_rshift r := {
   }. 
 
 Lemma rapply_red r i : Q_rapply r i =q=> rapply r i.
-Proof. funelim (rapply r i) ; triv. Qed.
+Proof. funelim (rapply r i) ; auto. Qed.
 #[local] Hint Rewrite <-rapply_red : red.
 
 (*********************************************************************************)
@@ -298,7 +282,7 @@ Proof.
 apply qclean_elim with 
   (P := fun i res => i =q=> res)
   (P0 := fun r res => r =r=> res).
-all: intros ; simp red ; triv.
+all: intros ; simp red ; auto.
 all: solve [ now rewrite <-H, <-H0 ].
 Qed.
 
@@ -317,13 +301,15 @@ Proof. now apply qrclean_red. Qed.
 (** Cleanup [E_sapply s i]. *)
 Equations sapply : subst -> qnat -> expr Kt :=
 sapply s i with dest_ren s := { 
-  | Some r => E_tvar (rapply r i)
+  | Some r => E_var (rapply r i)
   | None => E_sapply s i
   }. 
 
 Lemma sapply_red s i : E_sapply s i =e=> sapply s i.
 Proof. 
-funelim (sapply s i) ; simp red ; triv. etransitivity ; triv.
+funelim (sapply s i) ; simp red.
+- rewrite <-ered_ren_var. auto.
+- reflexivity.  
 Qed.
 #[local] Hint Rewrite <-sapply_red : red.
 
@@ -333,11 +319,11 @@ Qed.
 
 (** Cleanup [E_ren r t]. *)
 Equations rename {k} : ren -> expr k -> expr k :=
-rename r (E_tvar i) := E_tvar (rapply r i) ;
+rename r (E_var i) := E_var (rapply r i) ;
 rename r t := E_ren r t.
 
 Lemma rename_red {k} r (t : expr k) : E_ren r t =e=> rename r t.
-Proof. funelim (rename r t) ; simp red ; triv. Qed.
+Proof. funelim (rename r t) ; simp red ; easy. Qed.
 #[local] Hint Rewrite <-@rename_red : red.
 
 (*********************************************************************************)
@@ -346,14 +332,14 @@ Proof. funelim (rename r t) ; simp red ; triv. Qed.
 
 (** Cleanup [E_subst s t]. *)
 Equations substitute {k} : subst -> expr k -> expr k :=
-substitute s (E_tvar i) := sapply s i ;
+substitute s (E_var i) := sapply s i ;
 substitute s t with dest_ren s := {
   | Some r => rename r t 
   | None => E_subst s t
   }.
 
 Lemma substitute_red {k} s (t : expr k) : E_subst s t =e=> substitute s t.
-Proof. funelim (substitute s t) ; simp red ; triv. Qed.
+Proof. funelim (substitute s t) ; simp red ; auto ; try easy. Qed.
 #[local] Hint Rewrite <-@substitute_red : red.
 
 (*********************************************************************************)
@@ -361,13 +347,14 @@ Proof. funelim (substitute s t) ; simp red ; triv. Qed.
 (*********************************************************************************)
   
 Equations eclean {k} : expr k -> expr k :=
-eclean (E_tvar i) := E_tvar (qclean i) ;
-eclean (E_tctor c al) := E_tctor c (eclean al) ;
+eclean (E_var i) := E_var (qclean i) ;
+eclean (E_ctor c al) := E_ctor c (eclean al) ;
 eclean E_al_nil := E_al_nil ;
 eclean (E_al_cons a al) := E_al_cons (eclean a) (eclean al) ;
 eclean (E_abase b x) := E_abase b x ;
 eclean (E_aterm t) := E_aterm (eclean t) ;
 eclean (E_abind a) := E_abind (eclean a) ;
+eclean (E_afunctor f sh al) := E_afunctor f sh (vec_map eclean al) ;
 eclean (E_sapply s i) := sapply (sclean s) (qclean i) ;
 eclean (E_ren r t) := rename (rclean r) (eclean t) ;
 eclean (E_subst s t) := substitute (sclean s) (eclean t) ;
@@ -382,13 +369,12 @@ sclean (S_ren r) := S_ren (rclean r) ;
 sclean (S_mvar m) := S_mvar m.
 
 Lemma eclean_sclean_red : 
-  (forall k (t : expr k), t =e=> eclean t) * (forall s, s =s=> sclean s).
+  (forall k (t : expr k), t =e=> eclean t) /\ (forall s, s =s=> sclean s).
 Proof.
-apply eclean_elim with 
-  (P := fun k t res => t =e=> res) 
-  (P0 := fun s res => s =s=> res).
-all: intros ; simp red ; triv.
-all: solve [ now rewrite <-H | now rewrite <-H, <-H0 ].
+apply expr_subst_ind.
+all: intros ; simp eclean red ; auto ; try easy.
+all: try solve [ now rewrite <-H | now rewrite <-H, <-H0 ].
+f_equiv. intros i. simp vec_nth. 
 Qed. 
 
 Lemma eclean_red {k} (t : expr k) : t =e=> eclean t.
@@ -399,98 +385,5 @@ Lemma sclean_red s : s =s=> sclean s.
 Proof. now apply eclean_sclean_red. Qed.
 #[local] Hint Rewrite sclean_red : red.
 
-(*********************************************************************************)
-(** *** Confluence of the rewriting system. *)
-(*********************************************************************************)
+End WithSignature.
 
-Lemma qred_local_confluence x y i : 
-  i =q=>₁ x -> i =q=>₁ y -> exists i', x =q=> i' /\ y =q=> i'.
-Proof.
-intros Hx Hy. depelim Hx ; depelim Hy.
-rewrite H in H0. depelim H0. eexists ; split ; reflexivity.
-Qed.
-
-Lemma ered_local_confluence {k} (x y t : expr k) :
-  t =e=>₁ x -> t =e=>₁ y -> exists t', x =e=> t' /\ y =e=> t'.
-Proof.
-intros Hx Hy. depelim Hx ; depelim Hy.
-all: try solve [ eexists ; triv ].
-- rewrite H in H0. depelim H0. eexists ; triv.
-- exists (E_tvar (Q_rapply r i)). split ; triv. etransitivity ; triv.
-- exists (E_tvar (Q_rapply r i)). split ; triv. etransitivity ; triv.
-- rewrite H in H0. depelim H0. eexists ; triv.
-Qed.
-
-(*Definition confluent {A} (r : relation A) :=
-  forall t x, r t x -> forall y, r t y -> exists t', r x t' /\ r y t'. 
-
-Lemma qred_rred_confluence : confluent qred /\ confluent rred.
-Proof.
-unfold confluent. apply qred_rred_ind 
-  with (P := fun t x => forall y, t =q=> y -> exists t', x =q=> t' /\ y =q=> t').
-all: intros ; triv.
-- destruct (H0 _ H3) as (t' & ? & ?). destruct (H2 _ H4) as (t'' & ? & ?).
-  exists t''. split ; triv.
-- rename y0 into z.
-
-
-    
-(*********************************************************************************)
-(** *** Termination of the rewriting system. *)
-(*********************************************************************************)
-
-Equations qmeasure : qnat -> nat :=
-qmeasure Q_zero := 0 ;
-qmeasure (Q_succ i) := qmeasure i ;
-qmeasure (Q_rapply r i) := 1 + rmeasure r + qmeasure i ;
-qmeasure (Q_mvar _) := 0
-
-with rmeasure : ren -> nat :=
-rmeasure R_id := 0 ;
-rmeasure R_shift := 0 ;
-rmeasure (R_cons i r) := rmeasure r ;
-rmeasure (R_comp r1 r2) := rmeasure r1 + rmeasure r2 ;
-rmeasure (R_mvar _) := 0.
-
-Lemma mk_qsucc_measure n i : 
-  qmeasure (mk_qsucc n i) = qmeasure i.
-Proof. funelim (mk_qsucc n i) ; simp qmeasure ; lia. Qed.
-#[local] Hint Rewrite mk_qsucc_measure : qmeasure.
-
-(*Lemma dest_rshift_measure r n : 
-  dest_rshift r = Some n -> rmeasure r = 0.
-Proof.
-intros H. funelim (dest_rshift r) ; simp dest_rshift in * ; triv.
-- rewrite Heq, Heq0 in H. simp dest_rshift in H. depelim H. 
-  simp qmeasure. rewrite (Hind n2), (Hind0 n1) by assumption. lia.
-- rewrite Heq, Heq0 in H. simp dest_rshift in H. depelim H.
-- rewrite Heq in H. simp dest_rshift in H. depelim H.
-Qed.*)
-
-Lemma qred_rred_decreased : 
-  (forall i i', i =q=> i' -> qmeasure i' < qmeasure i) /\
-  (forall r r', r =r=> r' -> rmeasure r' < rmeasure r).
-Proof.
-apply qred_rred_ind ; intros ; simp qmeasure.
-all: try lia.
-- admit.
-- admit.
-Admitted.  
-
-Equations emeasure {k} : expr k -> nat :=
-emeasure (E_var _) := 0 ;
-emeasure (E_ctor c al) := emeasure al ;
-emeasure E_al_nil := 0 ;
-emeasure (E_al_cons a al) := emeasure a + emeasure al ;
-emeasure (E_abase _ _) := 0 ;
-emeasure (E_aterm t) := emeasure t ;
-emeasure (E_abind a) := emeasure a ;
-emeasure ()
-emeasure (Q_mvar _) := 0
-
-with rmeasure : ren -> nat :=
-rmeasure R_id := 0 ;
-rmeasure R_shift := 0 ;
-rmeasure (R_cons i r) := 1 + qmeasure i + rmeasure r ;
-rmeasure (R_comp r1 r2) := 1 + rmeasure r1 + rmeasure r2 ;
-rmeasure (R_mvar _) := 0.*)
