utils/Vector.v
@@ -8,8 +8,6 @@ From Utils Require Import Fin.
 (** Enable reducing constants defined using [Equations]. *)
 Set Equations Transparent.
 
-Set Universe Polymorphism.
-
 (*********************************************************************************)
 (** *** Vectors. *)
 (*********************************************************************************)
@@ -24,15 +22,19 @@ Arguments vcons {T n}.
 
 Derive Signature NoConfusion NoConfusionHom for vec.
 
-(** Notation for vectors, in scope [vec]. *)
+(*********************************************************************************)
+(** *** Notations for vectors. *)
+(*********************************************************************************)
 
-Declare Scope vec_scope.
-Bind Scope vec_scope with vec.
-Delimit Scope vec_scope with vec.
-
-Notation "[-  -]" := vnil : vec_scope. 
-Notation "[-  x  -]" := (vcons x vnil) : vec_scope.
-Notation "[-  x ; y ; .. ; z  -]" := (vcons x (vcons y .. (vcons z vnil) ..)) : vec_scope.
+Module VectorNotations.
+  Declare Scope vec_scope.
+  Bind Scope vec_scope with vec.
+  Delimit Scope vec_scope with vec.
+  
+  Notation "[  ]" := vnil : vec_scope. 
+  Notation "[  x  ]" := (vcons x vnil) : vec_scope.
+  Notation "[  x ; y ; .. ; z  ]" := (vcons x (vcons y .. (vcons z vnil) ..)) : vec_scope.
+End VectorNotations.
 
 (*********************************************************************************)
 (** *** Operations on vectors. *)
@@ -51,7 +53,7 @@ vec_nth (vcons x xs) finO     := x ;
 vec_nth (vcons x xs) (finS i) := vec_nth xs i.
 
 (** [vec_map f xs] maps function [f] over vector [xs]. *)
-Equations vec_map {T U n} (f : T -> U) (xs : vec T n) : vec U n :=
+Equations vec_map {T U} (f : T -> U) {n} (xs : vec T n) : vec U n :=
 vec_map f vnil := vnil ;
 vec_map f (vcons x xs) := vcons (f x) (vec_map f xs). 
 
@@ -62,32 +64,60 @@ vec_mapi f vnil := vnil ;
 vec_mapi f (vcons x xs) := vcons (f finO x) (vec_mapi (fun i => f (finS i)) xs). 
 
 (** [vec_map2 f xs ys] maps the binary function [f] over vectors [xs] and [ys]. *)
-Equations vec_map2 {T1 T2 U n} (f : T1 -> T2 -> U) (xs : vec T1 n) (ys : vec T2 n) : vec U n :=
+Equations vec_map2 {T1 T2 U} (f : T1 -> T2 -> U) {n} (xs : vec T1 n) (ys : vec T2 n) : vec U n :=
 vec_map2 f vnil vnil := vnil ;
 vec_map2 f (vcons x xs) (vcons y ys) := vcons (f x y) (vec_map2 f xs ys). 
+
+(** [vec_of_list xs] converts the list [xs] into a vector of length [List.length xs]. *)
+Equations vec_of_list {T} (xs : list T) : vec T (List.length xs) :=
+vec_of_list nil := vnil ;
+vec_of_list (cons x xs) := vcons x (vec_of_list xs).
+
+(** [list_of_vec xs] converts the vector [xs] into a list. *)
+Equations list_of_vec {T n} (xs : vec T n) : list T :=
+list_of_vec vnil := nil ;
+list_of_vec (vcons x xs) := x :: list_of_vec xs. 
+
+(** Compute the sum of a vector of [nat]. *)
+Equations vec_sum {n} (xs : vec nat n) : nat :=
+vec_sum vnil := 0 ;
+vec_sum (vcons x xs) := x + vec_sum xs. 
+
+(** [All_vec P xs] asserts that the predicate [P] is true on all elements of [xs]. *)
+Inductive All_vec {A} (P : A -> Prop) : forall {n}, vec A n -> Prop :=
+| All_vnil : All_vec P vnil
+| All_vcons n x (xs : vec A n) : P x -> All_vec P xs -> All_vec P (vcons x xs).
 
 (*********************************************************************************)
 (** *** Lemmas about vectors. *)
 (*********************************************************************************)
 
-Lemma vec_nth_mapi {n T U} (f : fin n -> T -> U) xs i :
+Lemma vec_nth_map {T U n} (f : T -> U) (xs : vec T n) i :
+  vec_nth (vec_map f xs) i = f (vec_nth xs i).
+Proof. funelim (vec_nth xs i) ; simp vec_map vec_nth. reflexivity. Qed.
+#[export] Hint Rewrite @vec_nth_map : vec_nth.
+
+Lemma vec_nth_mapi {T U n} (f : fin n -> T -> U) xs i :
   vec_nth (vec_mapi f xs) i = f i (vec_nth xs i).
 Proof. funelim (vec_nth xs i) ; simp vec_mapi vec_nth. reflexivity. Qed.
 #[export] Hint Rewrite @vec_nth_mapi : vec_nth.
 
-Lemma vec_nth_map2 {n T1 T2 U} (f : T1 -> T2 -> U) xs ys (i : fin n) :
+Lemma vec_nth_map2 {T1 T2 U n} (f : T1 -> T2 -> U) xs ys (i : fin n) :
   vec_nth (vec_map2 f xs ys) i = f (vec_nth xs i) (vec_nth ys i).
 Proof. 
 funelim (vec_nth xs i) ; depelim ys ; simp vec_map2 vec_nth. reflexivity.
 Qed.
 #[export] Hint Rewrite @vec_nth_map2 : vec_nth.
 
-Lemma vec_nth_init {n T} (f : fin n -> T) i :
+Lemma vec_nth_init {T n} (f : fin n -> T) i :
   vec_nth (vec_init n f) i = f i.
 Proof. 
 funelim (vec_init n f) ; depelim i ; simp vec_nth. reflexivity.
 Qed.
 #[export] Hint Rewrite @vec_nth_init : vec_nth.   
+
+Lemma list_vec_inv {T} (x : list T) : list_of_vec (vec_of_list x) = x.
+Proof. induction x ; [reflexivity | cbn ; now f_equal]. Qed. 
 
 (*********************************************************************************)
 (** *** Setoid rewrite support. *)
@@ -121,13 +151,39 @@ Section VecEq.
 
 End VecEq. 
 
-#[export] Instance vec_map_proper {T U n} (RT : relation T) (RU : relation U) : 
-  Proper ((RT ==> RU) ==> vec_eq RT ==> vec_eq RU) (@vec_map T U n). 
+Lemma vec_ext {T n} (xs xs' : vec T n) :
+  vec_eq eq xs xs' -> xs = xs'.
 Proof.
-intros f f' Hf xs xs' Hxs i. 
+intros H. induction n ; depelim xs ; depelim xs'.
+- reflexivity.
+- apply vec_eq_vcons_inv in H. f_equal.
+  + apply H.
+  + apply IHn, H.
+Qed.
+
+(* Because [n] of dependencies between arguments of [vec_map] we can't fully use
+   the pretty Proper notation. *)
+#[export] Instance vec_map_proper {T U} (RT : relation T) (RU : relation U) : 
+  let R : relation (forall n, vec T n -> vec U n) := fun f f' =>
+    forall n, (@vec_eq T RT n ==> @vec_eq U RU n)%signature (f n) (f' n)
+  in
+  Proper ((RT ==> RU) ==> R) (@vec_map T U). 
+Proof.
+cbn. intros f f' Hf n xs xs' Hxs i. 
 induction i ; depelim xs ; depelim xs' ; simp vec_nth vec_map.
 - apply Hf. now apply vec_eq_vcons_inv in Hxs.
-- apply IHi. now apply vec_eq_vcons_inv in Hxs.
+- apply Hf. now apply vec_eq_vcons_inv in Hxs.
+Qed.
+
+#[export] Instance vec_map_proper_ext {T U} : 
+  let R : relation ((T -> U) -> forall n, vec T n -> vec U n) := fun F F' =>
+    forall f f' n xs xs',
+    (forall i, f (vec_nth xs i) = f' (vec_nth xs' i)) -> 
+    F f n xs = F' f' n xs'
+  in
+  Proper R (@vec_map T U). 
+Proof.
+cbn. intros f f' n xs xs' H. apply vec_ext. intros i. simp vec_nth.
 Qed.
 
 #[export] Instance vec_mapi_proper {T U n} (RT : relation T) (RU : relation U) : 
@@ -141,7 +197,7 @@ induction i ; depelim xs ; depelim xs'.
   + now apply vec_eq_vcons_inv in Hxs.
 Qed.
 
-#[export] Instance vec_map2_proper {T1 T2 U n} 
+(*#[export] Instance vec_map2_proper {T1 T2 U n} 
   (RT1 : relation T1) (RT2 : relation T2) (RU : relation U) : 
   Proper ((RT1 ==> RT2 ==> RU) ==> vec_eq RT1 ==> vec_eq RT2 ==> vec_eq RU) 
     (@vec_map2 T1 T2 U n). 
@@ -154,4 +210,4 @@ induction i ; depelim xs ; depelim xs' ; depelim ys ; depelim ys' ; simp vec_nth
 - apply Hf. 
   + now apply vec_eq_vcons_inv in Hxs.
   + now apply vec_eq_vcons_inv in Hys.
-Qed.
+Qed.*)
