theories/Sig.v
@@ -2,24 +2,28 @@ From Prototype Require Import Prelude.
 
 (** This file defines the notion of abstract signature of a language. *)
 
-(** Argument types over a set of base types. *)
-Inductive arg_ty {base} :=
+(** Argument types over a set of base types and a set of functors. *)
+Inductive arg_ty {base fctor} :=
 | AT_base : base -> arg_ty
 | AT_term : arg_ty
-| AT_bind : arg_ty -> arg_ty.
+| AT_bind : arg_ty -> arg_ty
+| AT_functor : fctor -> arg_ty -> arg_ty.
+
 Derive NoConfusion NoConfusionHom for arg_ty.
 
-(** Kind of an expression (this is used in both level one and level two). *)
-Inductive kind {base} := 
+(** Kind of an expression (this is used in both parameterized syntax and 
+    explicit syntax). *)
+Inductive kind {base fctor} := 
 | (** Term. *)
   Kt : kind
 | (** Constructor argument. *)
-  Ka : @arg_ty base -> kind
+  Ka : @arg_ty base fctor -> kind
 | (** List of constructor arguments. *)
-  Kal : list (@arg_ty base) -> kind.
+  Kal : list (@arg_ty base fctor) -> kind.
+
 Derive NoConfusion NoConfusionHom for kind.
 
-(** Signatures for abstract terms. *)
+(** Signatures for abstract grammars. *)
 Record signature :=
 { (** The set of base types, 
       e.g. [Inductive base := BUnit | BBool | BNat]. *)
@@ -29,12 +33,34 @@ Record signature :=
 ; (** The actual type that each base type represents,
       e.g. a mapping BNat => nat ; BBool => bool ; BUnit => unit. *)
   eval_base : base -> Type
+
+; (** The set of _normal_ functors,
+      e.g. [Inductive fctor := FOption | FList]. *)
+  fctor : Type 
+; (** Decidable equality on [fctor]. *)
+  fctor_EqDec : EqDec fctor
+; (** Each normal functor must have a shape. *)
+  fctor_shape : fctor -> Type 
+; (** Each normal functor must have a size. *)
+  fctor_size : forall f, fctor_shape f -> nat
+
 ; (** The set of _non variable_ constructors, 
       e.g. [Inductive ctor := CApp | CLam]. *)
   ctor : Type
 ; (** Decidable equality on [ctor]. *)
   ctor_EqDec : EqDec ctor
 ; (** The number and types of the arguments of each constructor. *)
-  ctor_type : ctor -> list (@arg_ty base) }.
+  ctor_type : ctor -> list (@arg_ty base fctor) }.
+
+Arguments base {s}.
+Arguments base_EqDec {s}.
+Arguments eval_base {s}.
+Arguments fctor {s}.
+Arguments fctor_EqDec {s}.
+Arguments fctor_shape {s}.
+Arguments fctor_size {s}.
+Arguments ctor {s}.
+Arguments ctor_EqDec {s}.
+Arguments ctor_type {s}.
 
 Existing Class signature.
